compiler_test/bad_programs/out_of_bound_pointer.c
@@ -1,0 +1,15 @@
+#include <stdio.h>
+
+int main() {
+    int arr[5] = {1, 2, 3, 4, 5};
+    int *ptr = arr;
+
+    // Out-of-bounds read
+    printf("Out-of-bounds read: %d\n", *(ptr + 10));
+
+    // Out-of-bounds write
+    *(ptr + 10) = 100;
+    printf("Out-of-bounds write successful\n");
+
+    return 0;
+}
