cfrontend/BeePL_typesystem.v
@@ -18,9 +18,6 @@ Inductive type_expr : ty_context -> store_context -> expr -> effect -> type -> P
                type_expr Gamma Sigma (Val (Vint64 i) (Ptype (Tlong s a))) empty_effect (Ptype (Tlong s a))
 | Ty_val_loc : forall Gamma Sigma h t l ofs a,
                type_expr Gamma Sigma (Val (Vloc l ofs) (Reftype h (Bprim t) a)) empty_effect (Reftype h (Bprim t) a) 
-| Ty_valof : forall Gamma Sigma e t,
-             type_expr Gamma Sigma e empty_effect t  ->
-             type_expr Gamma Sigma (Valof e t) empty_effect t
 | Ty_var : forall Gamma Sigma x t, 
            PTree.get x.(vname) (extend_context Gamma x.(vname) t) = Some t ->
            x.(vtype) = t ->
@@ -95,9 +92,6 @@ Context (Htvall : forall Gamma Sigma i s a,
                   Pt Gamma Sigma (Val (Vint64 i) (Ptype (Tlong s a))) empty_effect (Ptype (Tlong s a))).
 Context (Htvalloc : forall Gamma Sigma h t l ofs a,
                     Pt Gamma Sigma (Val (Vloc l ofs) (Reftype h (Bprim t) a)) empty_effect (Reftype h (Bprim t) a)). 
-Context (Htvalof : forall Gamma Sigma e t,
-                   Pt Gamma Sigma e empty_effect t  ->
-                   Pt Gamma Sigma (Valof e t) empty_effect t).
 Context (Htvar : forall Gamma Sigma x t,
                  PTree.get x.(vname) (extend_context Gamma x.(vname) t) = Some t ->
                  x.(vtype) = t ->
@@ -159,8 +153,6 @@ Lemma type_expr_indP :
 (forall Gamma Sigma e ef t, type_expr Gamma Sigma e ef t -> Pt Gamma Sigma e ef t).
 Proof.
 apply type_exprs_type_expr_ind_mut=> //=.
-(* Valof *)
-+ move=> Gamma Sigma e t hte h. by apply Htvalof. 
 (* ConsInt *)
 + move=> Gamma Sigma t sz s a i. by apply Htconti.
 (* ConsLong *)
@@ -221,7 +213,6 @@ apply type_expr_indP => //=.
 + by move=> Gamma Sigma i sz s a ef' t' ht; inversion ht; subst.
 + by move=> Gamma Sigma i s a ef' t' ht; inversion ht; subst.
 + by move=> Gamma Sigma h t l ofs a ef' t' ht; inversion ht; subst.
-+ by move=> Gamma Sigma e t hi ef' t' ht; inversion ht; subst.
 + move=> Gamma Sigma x t htx ht ef' t' het; subst. by inversion het; subst.
 + move=> Gamma Sigma t sz s i a ht ef' t' ht'; subst. by inversion ht'; subst.
 + move=> Gamma Sigma t s i a ht ef' t' ht'; subst. by inversion ht'; subst.
@@ -432,81 +423,58 @@ Values.Val.has_type v (typ_of_type ct2).
 Proof.
 Admitted.
 
-(*Lemma type_transl_val : forall  t g ct g' i v v',
-transBeePL_type t g = SimplExpr.Res ct g' i ->
-Values.Val.has_type v (typ_of_type ct) ->
-transC_val_bplvalue v = Errors.OK v' ->
-typeof_value v' (wtype_of_type t).
-Proof.
-move=> t g ct g' i v v' /= hte hvt hv'. elim: t hte=> //=.
-+ move=> p. case: p=> //=.
-  + rewrite /SimplExpr.ret /=. move=> [] hct hg; subst.
-    rewrite /typ_of_type /= in hvt. case: v hv' hvt=> //= i'.
-    move=> [] hv' _; subst. rewrite /typeof_value /wtype_of_type /=.*)
-
-
 Section Subject_Reduction.
 
 Variable (bge : genv).
 Variable (benv : vmap).
 
 (* Subject reduction : Big step semantics *) 
-Lemma bsreduction_lreduction : 
-(forall m e l ofs,
-    bsem_expr_slv bge benv m e l ofs ->
-    forall Gamma Sigma ef t, 
-    type_expr Gamma Sigma e ef t ->
-    l.(ltype) = t) /\
-(forall m e v, 
-    bsem_expr_srv bge benv m e v ->
-    forall Gamma Sigma ef t, 
-     type_expr Gamma Sigma e ef t ->
-     typeof_value v (wtype_of_type t)).
+Lemma subject_lredcution : forall m e l ofs Gamma Sigma ef t,
+bsem_expr_slv bge benv m e l ofs ->
+type_expr Gamma Sigma e ef t ->
+l.(ltype) = t.
 Proof.
-apply bsem_expr_slv_rlv_ind=> //=.
-(* Var *)
-+ move=> m x t l h attr hx hv Gamma Sigma ef t' ht.
-  by inversion ht; subst.
-(* Gvar *)
-+ move=> m x t l h a hx hl hv Gamma Sigma ef t' ht.
-  by inversion ht; subst.
-(* Addr *)
-+ move=> m l ofs Gamma Sigma ef t ht. by inversion ht; subst.
-(* Deref *)
-+ move=> m e t l ofs hi Gamma Sigma ef t' ht. 
-  by inversion ht; subst.
+move=> m e l ofs Gamma Sigma ef t hl. 
+by induction hl=> //= ht; subst; inversion ht; subst; symmetry.
+Qed.
+
+Lemma subject_rreduction : forall m e v Gamma Sigma ef t, 
+bsem_expr_srv bge benv m e v ->
+type_expr Gamma Sigma e ef t ->
+typeof_value v (wtype_of_type t).
+Proof.
+move=> m e v Gamma Sigma ef t hr. move: Gamma Sigma ef t.
+induction hr=> //=. 
 (* Val *)
-+ move=> m v t Gamma Sigma ef t' ht. 
++ move=> Gamma Sigma ef t' ht. 
   by inversion ht; subst; rewrite /typeof_value /wtype_of_type.
 (* Const int *)
-+ move=> m i t Gamma Sigma ef t' ht. by inversion ht; subst; rewrite /wtype_of_type.
++ move=> Gamma Sigma ef t' ht. by inversion ht; subst; rewrite /wtype_of_type.
 (* Const long *)
-+ move=> m i t Gamma Sigma ef t' ht. by inversion ht; subst; rewrite /wtype_of_type.
-(* Valof *)
-+ move=> m e t l ofs v hi hd hte hvo Gamma Sigma ef t' ht.
-  inversion ht; subst.
-  move: (hi Gamma Sigma empty_effect (typeof_expr e) H5)=> hlt.
-  by have := deref_addr_val_ty (typeof_expr e) m l ofs v hd.
++ move=> Gamma Sigma ef t' ht. by inversion ht; subst; rewrite /wtype_of_type.
+(* Deref *)
++ move=> Gamma Sigma ef t' ht.
+  inversion ht; subst. rewrite H7.
+  have := subject_lredcution hm e l ofs Gamma Sigma ef0 (Reftype h (Bprim bt) a) H H9=> hlt.
+  by have := deref_addr_val_ty (typeof_expr e) hm l ofs v H0.
 (* Uop *)
-+ move=> m e v uop v' ct ct' v'' g g' i hi he hct hop hv Gamma Sigma ef t ht.
-  inversion ht; subst.
-  move: (hi Gamma Sigma ef (typeof_expr e) H6)=> hvt.
-  have hvt' := uop_type_preserve uop (transBeePL_value_cvalue v) ct' m v' hop.
-  by have := eq_uop_types uop (typeof_expr e) g g' i (transBeePL_value_cvalue v) ct' m v'
-          v'' he hop hvt' hv.
++ move=> Gamma Sigma ef t' ht. inversion ht; subst.
+  move: (IHhr Gamma Sigma ef (typeof_expr e) H10)=> hvt.
+  have hvt' := uop_type_preserve uop (transBeePL_value_cvalue v) ct hm v' H1.
+  by have := eq_uop_types uop (typeof_expr e) g g' i (transBeePL_value_cvalue v) ct hm v'
+          v'' H H1 hvt' H2.
 (* Bop *)
-+ move=> m e1 e2 t v1 v2 bop v ct1 ct2 v' g g' g'' i i' hi hi' hte1 hte2 
-         [] ht1 ht2 hop hv Gamma Sigma ef t' ht; subst. inversion ht; subst.
-  move: (hi Gamma Sigma ef t H7)=> hvt1. move: (hi' Gamma Sigma ef t H8)=> hvt2.
++ move=> Gamma Sigma ef t' ht; subst. inversion ht; subst.
+  move: (IHhr1 Gamma Sigma ef t0 H12)=> hvt1. move: (IHhr2 Gamma Sigma ef t0 H13)=> hvt2.
   have [hvt hvt'] := bop_type_preserve bge bop (transBeePL_value_cvalue v1) ct1 
-     (transBeePL_value_cvalue v2) ct2 m v hop.
-  by have := cval_bval_type_eq v ct1 v' (typeof_expr e1) g g' i hvt hv hte1.
+     (transBeePL_value_cvalue v2) ct2 hm v H2.
+  by have := cval_bval_type_eq v ct1 v' (typeof_expr e1) g g' i hvt H3 H; case: H1=> [] h1 h2; subst.
 Qed.
 
 
 End Subject_Reduction.
 
-(* Subject reduction *)
+(* Subject reduction : Small step semantics *)
 (* A well-typed expression remains well-typed under top-level lreduction *)
 Lemma slreduction : forall Gamma Sigma genv ef t vm e m e' m', 
 type_expr Gamma Sigma e ef t ->
@@ -517,9 +485,7 @@ move=> Gamma Sigma genv ef t vm e m e' m' ht he.
 induction he=> //=.
 + inversion ht; subst. rewrite H0. by apply Ty_addr with h t0 a. 
 + inversion ht; subst. rewrite H0. by apply Ty_addr with h t0 a.
-by inversion ht; subst.
 Qed.
-    
 
 
     
